reflectionScript.sml
@@ -416,8 +416,8 @@ bool_has_bool_interpretation
 |> SIMP_RULE std_ss [bool_model_models,bool_theory_ok]
 
 val _ = map2 (curry save_thm)
-  ["bool_theory_ok","bool_model_interpretation"]
-  [ bool_theory_ok , bool_model_interpretation ]
+  ["bool_theory_ok","bool_model_interpretation","bool_model_models"]
+  [ bool_theory_ok , bool_model_interpretation , bool_model_models]
 
 val not_thm = prove(
   ``is_set_theory ^mem ⇒
@@ -584,12 +584,36 @@ val _ = map2 (curry save_thm)
   ["in_fun_not","in_fun_forall","in_fun_exists","in_fun_binop","in_bool_false","in_bool_true"]
   [ in_fun_not , in_fun_forall , in_fun_exists , in_fun_binop , in_bool_false , in_bool_true ]
 
+val is_select_sig_def = Define`
+  is_select_sig sig ⇔
+  is_bool_sig sig ∧
+  (FLOOKUP (tmsof sig) "@" = SOME (Fun (Fun (Tyvar "A") Bool) (Tyvar "A")))`
+
+val select_sig_instances = store_thm("select_sig_instances",
+  ``is_select_sig sig ⇒
+    (instance (tmsof sig) i "@" (Fun (Fun ty Bool) ty) =
+       (λτ. tmaof i "@" [typesem (tyaof i) τ ty]))``,
+  rw[is_select_sig_def] >>
+  Q.ISPECL_THEN[`tmsof sig`,`i`,`"@"`]mp_tac instance_def >> simp[] >>
+  disch_then(qspec_then`[ty,Tyvar "A"]`mp_tac) >>
+  EVAL_TAC >> rw[])
+
+val select_has_select_sig = store_thm("select_has_select_sig",
+  ``is_bool_sig (sigof ctxt) ⇒ is_select_sig (sigof (mk_select_ctxt ctxt))``,
+  rw[is_select_sig_def] >- (
+    fs[is_bool_sig_def,mk_select_ctxt_def,FLOOKUP_UPDATE] >>
+    fs[is_std_sig_def,FLOOKUP_UPDATE] ) >>
+  EVAL_TAC)
+
 val select_model_exists = prove(
-  ``∃f. ∀mem. is_set_theory mem ⇒
-      subinterpretation (mk_bool_ctxt init_ctxt) (bool_model0 mem) (f mem) ∧
-      f mem models thyof (mk_select_ctxt (mk_bool_ctxt init_ctxt))``,
+  ``∃f. ∀mem select. is_set_theory mem ⇒ good_select select ⇒
+      subinterpretation (mk_bool_ctxt init_ctxt) (bool_model0 mem) (f mem select) ∧
+      f mem select models thyof (mk_select_ctxt (mk_bool_ctxt init_ctxt)) ∧
+      (tmaof (f mem select) "@" = λls.
+        Abstract (Funspace (HD ls) boolset) (HD ls)
+          (λp. select (HD ls) (Holds p)))``,
   rw[GSYM SKOLEM_THM,RIGHT_EXISTS_IMP_THM] >>
-  qspec_then`mk_bool_ctxt init_ctxt`mp_tac(UNDISCH select_has_model) >>
+  qspec_then`mk_bool_ctxt init_ctxt`mp_tac(UNDISCH select_has_model_gen) >>
   discharge_hyps_keep >- (
     simp[bool_theory_ok] >>
     EVAL_TAC ) >>
@@ -601,7 +625,7 @@ val select_model_exists = prove(
 val select_model_def = new_specification("select_model_def",["select_model0"],
   select_model_exists)
 val _ = overload_on("select_model",``select_model0 ^mem``)
-val select_model_models = UNDISCH (SPEC mem select_model_def)
+val select_model_models = GEN_ALL (UNDISCH (SPEC_ALL (SPEC mem select_model_def)))
 
 val select_extends_bool = prove(
   ``mk_select_ctxt (mk_bool_ctxt init_ctxt) extends mk_bool_ctxt init_ctxt``,
@@ -619,15 +643,16 @@ extends_theory_ok
 
 val select_bool_interpretation = prove(
   ``is_set_theory ^mem ⇒
-    is_bool_interpretation select_model``,
+    good_select select ⇒
+    is_bool_interpretation (select_model select)``,
   rw[] >>
-  assume_tac select_model_models >>
+  first_assum(strip_assume_tac o MATCH_MP select_model_models) >>
   assume_tac bool_model_interpretation >>
   fs[subinterpretation_def,is_bool_interpretation_def] >>
   conj_tac >- ( fs[models_def] ) >>
   fs[term_ok_def] >>
   rpt conj_tac >>
-  qmatch_abbrev_tac`tmaof select_model interprets name on args as val` >>
+  qmatch_abbrev_tac`tmaof (select_model select) interprets name on args as val` >>
   first_x_assum(qspec_then`name`mp_tac) >>
   qunabbrev_tac`name` >>
   CONV_TAC(LAND_CONV(QUANT_CONV(LAND_CONV EVAL))) >>
@@ -637,22 +662,22 @@ val select_bool_interpretation = prove(
        metis_tac[base_tyval_def] ) >>
   fs[PULL_EXISTS,type_ok_def,FLOOKUP_UPDATE] >>
   first_x_assum(qspec_then`[]`mp_tac)>>
-  (discharge_hyps >- EVAL_TAC) >> rw[]) |> UNDISCH
+  (discharge_hyps >- EVAL_TAC) >> rw[]) |> UNDISCH |> UNDISCH
 
 val _ = map2 (curry save_thm)
-  ["select_theory_ok","select_extends_bool","select_bool_interpretation"]
-  [ select_theory_ok , select_extends_bool , select_bool_interpretation ]
+  ["select_theory_ok","select_extends_bool","select_bool_interpretation","select_model_models"]
+  [ select_theory_ok , select_extends_bool , select_bool_interpretation , select_model_models ]
 
 val constrained_term_valuation_exists = store_thm("constrained_term_valuation_exists",
   ``is_set_theory ^mem ⇒
-    ∀tyenv δ τ.  is_type_valuation τ ⇒ is_type_assignment tyenv δ ⇒
+    ∀tysig δ τ.  is_type_valuation τ ⇒ is_type_assignment tysig δ ⇒
     ∀constraints.
     ALL_DISTINCT (MAP FST constraints) ∧
-    EVERY (λ(k,v). type_ok tyenv (SND k) ∧
+    EVERY (λ(k,v). type_ok tysig (SND k) ∧
                    v <: typesem δ τ (SND k)) constraints
     ⇒
     ∃σ.
-      is_term_valuation tyenv δ τ σ ∧
+      is_term_valuation tysig δ τ σ ∧
       EVERY (λ(k,v). σ k = v) constraints``,
   strip_tac >> ntac 3 gen_tac >> ntac 2 strip_tac >> Induct >> simp[] >-
     metis_tac[term_valuation_exists,is_valuation_def,FST,SND] >>
@@ -684,6 +709,14 @@ val interprets_one = store_thm("interprets_one",
   first_x_assum(qspec_then`K x`mp_tac) >>
   simp[] >> disch_then match_mp_tac >>
   rw[is_type_valuation_def] >> metis_tac[])
+
+(* TODO: move *)
+
+val boolean_of_eq_true = store_thm("boolean_of_eq_true",
+  ``is_set_theory ^mem ⇒
+    ∀b. b <: boolset ⇒ (Boolean (b = True) = b)``,
+  rw[boolean_def] >> rw[] >>
+  metis_tac[mem_boolset])
 
 val is_std_sig_extends = store_thm("is_std_sig_extends",
   ``∀ctxt1 ctxt2. ctxt2 extends ctxt1 ⇒ is_std_sig (sigof ctxt1) ⇒ is_std_sig (sigof ctxt2)``,
